[language][prover] Added a test and fixed some bugs related to vectors.
1. Added basic tests test_mvir/verify-vector.mvir
2. Fixed an off-by-one error in src/prelude.bpl: RemoveValueArray
3. Added Boogie command-line option "-useArrayTheory" because Z3 array
extension we rely on need it. Otherwise, Boogie does not set invalid
elements of arrays to DefaultValue
4. Added a new variant ErrorType() to TypeValue and a new variant
Error() to Value, and added axioms to make the DefaultTypeValue=ErrorType()
and DefaultValue=Error().  The purpose of this change is to make it a little
easier to understand Boogie counter-models -- otherwise, Boogie assigns
random values that change with every change to the .bpl file, making it
much harder to see errors.
5. Added some short instructions for generating output.bpl in README.md.
I expect that this will be short-lived because there will be a better way.

language/move-prover/bytecode-to-boogie/src/cli.rs
@@ -17,8 +17,10 @@ use std::sync::atomic::{AtomicBool, Ordering};
 pub const INLINE_PRELUDE: &str = "<inline-prelude>";
 
 /// Default flags passed to boogie. Additional flags will be added to this via the -B option.
+
 const DEFAULT_BOOGIE_FLAGS: &[&str] = &[
     "-doModSetAnalysis",
+    "-useArrayTheory",
     "-noinfer",
     "-printVerifiedProceduresCount:0",
 ];
