language/move-prover/bytecode-to-boogie/tests/goldenfiles/verify-vector.bpl
@@ -1,0 +1,163 @@
+
+
+// ** structs of module VerifyVector
+
+
+
+// ** functions of module VerifyVector
+
+procedure {:inline 1} VerifyVector_test_empty1 () returns (ret0: Value, ret1: Value)
+requires ExistsTxnSenderAccount(m, txn);
+ensures b#Boolean(Boolean((ret0) == (ret1)));
+{
+    // declare local variables
+    var t0: Value; // Vector_T_type_value(IntegerType())
+    var t1: Value; // Vector_T_type_value(IntegerType())
+    var t2: Value; // Vector_T_type_value(IntegerType())
+    var t3: Value; // Vector_T_type_value(IntegerType())
+    var t4: Value; // Vector_T_type_value(IntegerType())
+    var t5: Value; // Vector_T_type_value(IntegerType())
+
+    var tmp: Value;
+    var old_size: int;
+
+    var saved_m: Memory;
+    assume !abort_flag;
+    saved_m := m;
+
+    // assume arguments are of correct types
+
+    old_size := local_counter;
+    local_counter := local_counter + 6;
+
+    // bytecode translation starts here
+    call t2 := Vector_empty(IntegerType());
+    if (abort_flag) { goto Label_Abort; }
+    assume is#Vector(t2);
+
+    m := UpdateLocal(m, old_size + 2, t2);
+
+    call tmp := CopyOrMoveValue(GetLocal(m, old_size + 2));
+    m := UpdateLocal(m, old_size + 0, tmp);
+
+    call t3 := Vector_empty(IntegerType());
+    if (abort_flag) { goto Label_Abort; }
+    assume is#Vector(t3);
+
+    m := UpdateLocal(m, old_size + 3, t3);
+
+    call tmp := CopyOrMoveValue(GetLocal(m, old_size + 3));
+    m := UpdateLocal(m, old_size + 1, tmp);
+
+    call tmp := CopyOrMoveValue(GetLocal(m, old_size + 0));
+    m := UpdateLocal(m, old_size + 4, tmp);
+
+    call tmp := CopyOrMoveValue(GetLocal(m, old_size + 1));
+    m := UpdateLocal(m, old_size + 5, tmp);
+
+    ret0 := GetLocal(m, old_size + 4);
+    ret1 := GetLocal(m, old_size + 5);
+    return;
+
+Label_Abort:
+    abort_flag := true;
+    m := saved_m;
+    ret0 := DefaultValue;
+    ret1 := DefaultValue;
+}
+
+procedure VerifyVector_test_empty1_verify () returns (ret0: Value, ret1: Value)
+{
+    assume ExistsTxnSenderAccount(m, txn);
+    call ret0, ret1 := VerifyVector_test_empty1();
+}
+
+procedure {:inline 1} VerifyVector_test_empty2 () returns (ret0: Value, ret1: Value)
+requires ExistsTxnSenderAccount(m, txn);
+ensures b#Boolean(Boolean((ret0) == (ret1)));
+{
+    // declare local variables
+    var t0: Value; // Vector_T_type_value(IntegerType())
+    var t1: Value; // Vector_T_type_value(IntegerType())
+    var t2: Value; // IntegerType()
+    var t3: Value; // Vector_T_type_value(IntegerType())
+    var t4: Value; // Vector_T_type_value(IntegerType())
+    var t5: Reference; // ReferenceType(Vector_T_type_value(IntegerType()))
+    var t6: Value; // IntegerType()
+    var t7: Reference; // ReferenceType(Vector_T_type_value(IntegerType()))
+    var t8: Value; // IntegerType()
+    var t9: Value; // Vector_T_type_value(IntegerType())
+    var t10: Value; // Vector_T_type_value(IntegerType())
+
+    var tmp: Value;
+    var old_size: int;
+
+    var saved_m: Memory;
+    assume !abort_flag;
+    saved_m := m;
+
+    // assume arguments are of correct types
+
+    old_size := local_counter;
+    local_counter := local_counter + 11;
+
+    // bytecode translation starts here
+    call t3 := Vector_empty(IntegerType());
+    if (abort_flag) { goto Label_Abort; }
+    assume is#Vector(t3);
+
+    m := UpdateLocal(m, old_size + 3, t3);
+
+    call tmp := CopyOrMoveValue(GetLocal(m, old_size + 3));
+    m := UpdateLocal(m, old_size + 0, tmp);
+
+    call t4 := Vector_empty(IntegerType());
+    if (abort_flag) { goto Label_Abort; }
+    assume is#Vector(t4);
+
+    m := UpdateLocal(m, old_size + 4, t4);
+
+    call tmp := CopyOrMoveValue(GetLocal(m, old_size + 4));
+    m := UpdateLocal(m, old_size + 1, tmp);
+
+    call t5 := BorrowLoc(old_size+0);
+
+    call tmp := LdConst(1);
+    m := UpdateLocal(m, old_size + 6, tmp);
+
+    call Vector_push_back(IntegerType(), t5, GetLocal(m, old_size + 6));
+    if (abort_flag) { goto Label_Abort; }
+
+    call t7 := BorrowLoc(old_size+0);
+
+    call t8 := Vector_pop_back(IntegerType(), t7);
+    if (abort_flag) { goto Label_Abort; }
+    assume IsValidU64(t8);
+
+    m := UpdateLocal(m, old_size + 8, t8);
+
+    call tmp := CopyOrMoveValue(GetLocal(m, old_size + 8));
+    m := UpdateLocal(m, old_size + 2, tmp);
+
+    call tmp := CopyOrMoveValue(GetLocal(m, old_size + 0));
+    m := UpdateLocal(m, old_size + 9, tmp);
+
+    call tmp := CopyOrMoveValue(GetLocal(m, old_size + 1));
+    m := UpdateLocal(m, old_size + 10, tmp);
+
+    ret0 := GetLocal(m, old_size + 9);
+    ret1 := GetLocal(m, old_size + 10);
+    return;
+
+Label_Abort:
+    abort_flag := true;
+    m := saved_m;
+    ret0 := DefaultValue;
+    ret1 := DefaultValue;
+}
+
+procedure VerifyVector_test_empty2_verify () returns (ret0: Value, ret1: Value)
+{
+    assume ExistsTxnSenderAccount(m, txn);
+    call ret0, ret1 := VerifyVector_test_empty2();
+}
