language/move-prover/README.md
@@ -1,9 +1,15 @@
 ---
 id: move-prover
 title: Formal verification code
-custom_edit_url: https://github.com/libra/libra/edit/master/language/README.md
+custom_edit_url: https://github.com/libra/libra/edit/master/language/move-prover/README.md
 ---
 
 # Code supporting formal verification for Move programs
 
 ## Code under this subtree is experimental. It is out of scope for [the Libra Bug Bounty](https://hackerone.com/libra) until it is no longer marked experimental.
+
+## Debugging tips
+
+During development, we sometimes want to edit the boogie file and run boogie on it explicitly.  You can see the boogie command line by cd'ing to the bytecode-to-boogie subdirectory and typing something like:
+
+cargo run -- --verbose debug ../../stdlib/modules/vector.mvir test_mvir/verify_vector.mvir
